An example of TM from Cook_Levin: A copy-paste machine that copies the 0th tape to the 1st tape

IMPminus-TM/Docs/TM_Playground.thy
@@ -4,6 +4,96 @@ theory TM_Playground
   imports Cook_Levin.Basics "IMP_Minus.AExp"
 begin
 
+subsection \<open>Helper functions\<close>
 
+text \<open>For a given config, print the first m symbols of n-th tape\<close>
+fun print_tape :: "config \<Rightarrow> nat \<Rightarrow> nat \<Rightarrow> symbol list" where
+  "print_tape cfg n 0 = []" |
+  "print_tape cfg n (Suc m) = (print_tape cfg n m) @ [(cfg <:> n) m]"
+
+subsection \<open>Example 1: copy-paste machine\<close>
+
+text \<open>A minimum machine that copies the 0-th (read-only) tape to the 1st tape
+With only two states: q_0 and q_f
+In q_0, it copies the symbol from the 0-th tape to the 1st tape,
+then moves the head one step to right on both tapes, remains in state q_0, iff the symbol is not \<box>;
+otherwise when then symbol from the 0-th tape is \<box>, it copies it as well to the 1st tape,
+then turn to state q_f (and terminates)
+\<close>
+
+definition copy_paste_command :: command where
+  "copy_paste_command = (
+    \<lambda> symbols_read_from_tapes.
+      (if symbols_read_from_tapes ! 0 = \<box> then 1 else 0, \<comment> \<open>new state\<close>
+       [(symbols_read_from_tapes ! 0, Right), \<comment> \<open>0-th tape remains the same\<close>
+        (symbols_read_from_tapes ! 0, Right)]) \<comment> \<open>copies the symbol from 0-th tape to the 1st tape\<close>
+   )"
+
+\<comment> \<open>copy_paste_command is a well-formed command for a 2-tape TM with 1 state (excluding q_f)\<close>
+lemma "wf_command 2 1 copy_paste_command"
+  unfolding copy_paste_command_def
+  unfolding wf_command_def
+  by simp
+
+
+\<comment> \<open>copy_paste_command is a Turing command for a 2-tape TM with 1 state (excluding q_f),
+    and with the alphabet set containing only one symbol (\<box>)\<close>
+lemma "turing_command 2 1 1 copy_paste_command"
+  unfolding copy_paste_command_def
+  unfolding turing_command_def
+  unfolding wf_command_def
+  apply auto
+  by (metis One_nat_def diff_Suc_1 fst_conv less_2_cases_iff nth_Cons_0 nth_Cons_numeral numerals(1))
+
+\<comment> \<open>Same as above,
+    and with the alphabet set containing only 4 symbols (\<box>, \<triangleright>, \<zero>, \<one>)\<close>
+lemma cp_tm_cmd_214: "turing_command 2 1 4 copy_paste_command"
+  unfolding copy_paste_command_def
+  unfolding turing_command_def
+  unfolding wf_command_def
+  apply auto
+  by (metis One_nat_def diff_Suc_1 fst_conv less_2_cases_iff nth_Cons_0 nth_Cons_numeral numerals(1))
+
+\<comment> \<open>And so on, this works for any size of the alphabet set as long as it is not empty\<close>
+thm turing_command_mono
+lemma "turing_command 2 1 100 copy_paste_command"
+  unfolding copy_paste_command_def
+  unfolding turing_command_def
+  unfolding wf_command_def
+  apply auto
+  by (metis One_nat_def diff_Suc_1 fst_conv less_2_cases_iff nth_Cons_0 nth_Cons_numeral numerals(1))
+
+
+definition copy_paste_machine :: machine where
+  "copy_paste_machine = [copy_paste_command]" \<comment> \<open>The behavior under each states except for q_f\<close>
+                                              \<comment> \<open>In this case, only for q_0\<close>
+
+\<comment> \<open>The copy-paste machine is a well-formed 2-tape TM for the alphabet set of size 4\<close>
+lemma "turing_machine 2 4 copy_paste_machine"
+  unfolding turing_machine_def copy_paste_machine_def
+  using cp_tm_cmd_214 by auto
+
+\<comment> \<open>An example of the executing of the copy-paste machine.
+    Start configuration: the 0-th tape has 5 \<triangleright>'s and then \<box>'s on it;
+    The 1st tape is full of \<box>'s.
+    Showing the first 10 symbols on the 1st tape after each of the first 8 steps.\<close>
+value "print_tape (execute copy_paste_machine (0, [(\<lambda>n. if n \<ge> 5 then \<box> else \<triangleright>, 0), (\<lambda>n. \<box>, 0)]) 0) 1 10"
+value "print_tape (execute copy_paste_machine (0, [(\<lambda>n. if n \<ge> 5 then \<box> else \<triangleright>, 0), (\<lambda>n. \<box>, 0)]) 1) 1 10"
+value "print_tape (execute copy_paste_machine (0, [(\<lambda>n. if n \<ge> 5 then \<box> else \<triangleright>, 0), (\<lambda>n. \<box>, 0)]) 2) 1 10"
+value "print_tape (execute copy_paste_machine (0, [(\<lambda>n. if n \<ge> 5 then \<box> else \<triangleright>, 0), (\<lambda>n. \<box>, 0)]) 3) 1 10"
+value "print_tape (execute copy_paste_machine (0, [(\<lambda>n. if n \<ge> 5 then \<box> else \<triangleright>, 0), (\<lambda>n. \<box>, 0)]) 4) 1 10"
+value "print_tape (execute copy_paste_machine (0, [(\<lambda>n. if n \<ge> 5 then \<box> else \<triangleright>, 0), (\<lambda>n. \<box>, 0)]) 5) 1 10"
+value "print_tape (execute copy_paste_machine (0, [(\<lambda>n. if n \<ge> 5 then \<box> else \<triangleright>, 0), (\<lambda>n. \<box>, 0)]) 6) 1 10"
+value "print_tape (execute copy_paste_machine (0, [(\<lambda>n. if n \<ge> 5 then \<box> else \<triangleright>, 0), (\<lambda>n. \<box>, 0)]) 7) 1 10"
+\<comment> \<open>Same example as above, showing the state after each of the first 8 steps.\<close>
+value "fst (execute copy_paste_machine (0, [(\<lambda>n. if n \<ge> 5 then \<box> else \<triangleright>, 0), (\<lambda>n. \<box>, 0)]) 0)"
+value "fst (execute copy_paste_machine (0, [(\<lambda>n. if n \<ge> 5 then \<box> else \<triangleright>, 0), (\<lambda>n. \<box>, 0)]) 1)"
+value "fst (execute copy_paste_machine (0, [(\<lambda>n. if n \<ge> 5 then \<box> else \<triangleright>, 0), (\<lambda>n. \<box>, 0)]) 2)"
+value "fst (execute copy_paste_machine (0, [(\<lambda>n. if n \<ge> 5 then \<box> else \<triangleright>, 0), (\<lambda>n. \<box>, 0)]) 3)"
+value "fst (execute copy_paste_machine (0, [(\<lambda>n. if n \<ge> 5 then \<box> else \<triangleright>, 0), (\<lambda>n. \<box>, 0)]) 4)"
+value "fst (execute copy_paste_machine (0, [(\<lambda>n. if n \<ge> 5 then \<box> else \<triangleright>, 0), (\<lambda>n. \<box>, 0)]) 5)"
+value "fst (execute copy_paste_machine (0, [(\<lambda>n. if n \<ge> 5 then \<box> else \<triangleright>, 0), (\<lambda>n. \<box>, 0)]) 6)"
+value "fst (execute copy_paste_machine (0, [(\<lambda>n. if n \<ge> 5 then \<box> else \<triangleright>, 0), (\<lambda>n. \<box>, 0)]) 7)"
+value "fst (execute copy_paste_machine (0, [(\<lambda>n. if n \<ge> 5 then \<box> else \<triangleright>, 0), (\<lambda>n. \<box>, 0)]) 8)"
 
 end
